Setlec/Verify/InferLeaves.lean
@@ -810,7 +810,7 @@ theorem inferTypeCore_WScoped {env : Env} (henv : EnvWF env) :
       exact WScoped.instantiate1_gen hw.2 0 hwPi.2
     | proj sn i pe =>
       obtain ⟨tpe, te, T, us, entry, hte, hwt, hfn, hfp, hnat, hlen,
-        hus, hres⟩ := inferTypeCore_proj_inv h
+        hus, -, hres⟩ := inferTypeCore_proj_inv h
       simp only [WScoped] at hw
       have hwte := inferTypeCore_WScoped henv fuel hte hw
       have hwPi := whnf_WScoped henv fuel hwt hwte
@@ -943,7 +943,7 @@ theorem inferTypeCore_fvarLeaves {env : Env} (henv : EnvWF env) :
       · exact Or.inr hb
     | proj sn i pe =>
       obtain ⟨tpe, te, T, us, entry, hte, hwt, hfn, hfp, hnat, hlen,
-        hus, hres⟩ := inferTypeCore_proj_inv h
+        hus, -, hres⟩ := inferTypeCore_proj_inv h
       simp only [WScoped] at hw
       intro l hl
       simp only [fvarLeaves]
@@ -1081,7 +1081,7 @@ theorem inferTypeCore_looseBVars {env : Env} (henv : EnvWF env) :
       exact looseBVarsBounded_instantiate1_gen hb.2 hbPi.2
     | proj sn i pe =>
       obtain ⟨tpe, te, T, us, entry, hte, hwt, hfn, hfp, hnat, hlen,
-        hus, hres⟩ := inferTypeCore_proj_inv h
+        hus, -, hres⟩ := inferTypeCore_proj_inv h
       simp only [WScoped] at hw
       simp only [looseBVarsBounded] at hb
       have hLbe : Expr.LeavesBounded pe := fun l hl => hLb l (by
